byteback-core/src/integration/java/byteback/core/converter/soottoboogie/ProcedureConverterIntegrationTest.java
@@ -1,0 +1,67 @@
+package byteback.core.converter.soottoboogie;
+
+import static org.junit.Assert.assertEquals;
+
+import byteback.core.RegressionParameter;
+import byteback.core.converter.soottoboogie.method.procedure.ProcedureConverter;
+import byteback.core.representation.soot.unit.SootClass;
+import byteback.frontend.boogie.ast.ConstantDeclaration;
+import byteback.frontend.boogie.ast.PrintUtil;
+import byteback.frontend.boogie.ast.Procedure;
+import byteback.frontend.boogie.ast.ProcedureDeclaration;
+import byteback.frontend.boogie.ast.Program;
+import java.io.IOException;
+import java.util.Optional;
+import java.util.stream.Stream;
+import org.junit.AfterClass;
+import org.junit.Test;
+import org.junit.runner.RunWith;
+import org.junit.runners.Parameterized;
+import org.junit.runners.Parameterized.Parameters;
+
+@RunWith(Parameterized.class)
+public class ProcedureConverterIntegrationTest extends ConverterFixture {
+
+	@AfterClass
+	public static void after() {
+		resetContext();
+	}
+
+	@Parameters
+	public static Iterable<RegressionParameter<ProcedureDeclaration>> getParameters() throws IOException {
+		return getRegressionEntries("java8").flatMap((entry) -> {
+			final SootClass clazz = entry.getKey();
+			final Program program = entry.getValue();
+
+			return clazz.methods().flatMap((method) -> {
+				if (!method.getAnnotation(Annotations.PURE_ANNOTATION).isPresent()
+						&& !method.getAnnotation(Annotations.CONDITION_ANNOTATION).isPresent()) {
+					final String name = NameConverter.methodName(method);
+					final Optional<ProcedureDeclaration> expected = program.lookupProcedure(name)
+							.map(Procedure::getProcedureDeclaration);
+
+					if (expected.isPresent()) {
+						final ProcedureDeclaration actual = ProcedureConverter.instance().convert(method);
+
+						return Stream.of(new RegressionParameter<>(expected.get(), actual));
+					}
+				}
+
+				return Stream.empty();
+			});
+		})::iterator;
+	}
+
+	private final RegressionParameter<ConstantDeclaration> parameter;
+
+	public ProcedureConverterIntegrationTest(final RegressionParameter<ConstantDeclaration> parameter) {
+		this.parameter = parameter;
+	}
+
+	@Test
+	public void Convert_GivenRegressionSet_ReturnsExpectedCode() {
+    System.err.println(PrintUtil.toString(parameter.actual));
+		assertEquals(PrintUtil.toString(parameter.expected), PrintUtil.toString(parameter.actual));
+	}
+
+}
