byteback-core/src/main/java/byteback/core/converter/soottoboogie/method/function/FunctionConverter.java
@@ -69,8 +69,6 @@ public class FunctionConverter {
 	public FunctionDeclaration convert(final SootMethod method) {
 		final var functionBuilder = new FunctionDeclarationBuilder();
 
-    System.out.println(method.getBody());
-
     try {
 			functionBuilder.name(NameConverter.methodName(method));
 			buildSignature(functionBuilder, method);
