byteback-core/src/integration/resources/regression/java8/boogie/byteback.dummy.condition.Array.bpl
@@ -1,90 +1,7 @@
-// -------------------------------------------------------------------
-// Heap model
-// -------------------------------------------------------------------
-type Reference;
-
-const ~null: Reference;
-
-type Field a;
-type Store = [Reference]<a>[Field a]a;
-
-var ~heap: Store;
-
-function ~read<a>(h: Store, r: Reference, f: Field a) returns (a)
-{ h[r][f] }
-
-function ~update<a>(h: Store, r: Reference, f: Field a, v: a) returns (Store)
-{ h[r := h[r][f := v]] }
-
-procedure ~new() returns (~ret: Reference);
-
-// -------------------------------------------------------------------
-// Array model
-// -------------------------------------------------------------------
-type Array a = Field [int]a;
-
-const unique ~Array.bool: Array bool;
-
-const unique ~Array.int: Array int;
-
-const unique ~Array.real: Array real;
-
-const unique ~Array.Reference: Array Reference;
-
-const unique ~Array.length: Field int;
-
-function ~lengthof(h: Store, r: Reference) returns (int)
-{
-  ~read(h, r, ~Array.length)
-}
-
-function ~get<a>(h: Store, r: Reference, f: Array a, i: int) returns (a)
-{
-  ~read(h, r, f)[i]
-}
-
-function ~insert<a>(h: Store, r: Reference, f: Array a, i: int, e: a) returns (Store)
-{
-  ~update(h, r, f, ~read(h, r, f)[i := e])
-}
-
-procedure ~array(l: int) returns (~ret: Reference);
-  modifies ~heap;
-  ensures ~read(~heap, ~ret, ~Array.length) == l;
-
-// -------------------------------------------------------------------
-// Binary operators
-// -------------------------------------------------------------------
-function ~cmp<a>(a, a) returns (int);
-
-axiom (forall i: int, j: int :: i < j ==> ~cmp(i, j) == -1);
-axiom (forall i: int, j: int :: i > j ==> ~cmp(i, j) == 1);
-axiom (forall i: int, j: int :: i == j ==> ~cmp(i, j) == 0);
-
-axiom (forall i: real, j: real :: i < j ==> ~cmp(i, j) == -1);
-axiom (forall i: real, j: real :: i > j ==> ~cmp(i, j) == 1);
-axiom (forall i: real, j: real :: i == j ==> ~cmp(i, j) == 0);
-
-// -------------------------------------------------------------------
-// Casting operators
-// -------------------------------------------------------------------
-
-// Casting between primitive types
-function ~int<a>(a) returns (int);
-
-// bool -> int
-axiom ~int(false) == 0;
-axiom ~int(true) == 1;
-
-// real -> int
-// TODO
-
-function ~real<a>(a) returns (real);
-
-// int -> real
-// TODO
-
 procedure byteback.dummy.condition.Array.sum#int$#(as: Reference) returns (~ret: int)
+  ensures ~implies(~heap,
+    (forall index: int :: ~and(~heap, ~lt(~heap, index, ~lengthof(~heap, as)), ~gte(~heap, index, 0))),
+    ~gte(~heap, ~ret, 0));
 {
   var c: int;
   var l4: int;
@@ -110,6 +27,7 @@ label1:
 }
 
 procedure byteback.dummy.condition.Array.assignsLastElement#int$#(as: Reference) returns ()
+  ensures ~eq(~heap, ~get(~heap, as, ~Array.int, ~lengthof(~heap, as) - 1), 1);
 {
   ~heap := ~insert(~heap, as, ~Array.int, ~lengthof(~heap, as) - 1, 1);
   return;
