byteback-core/src/integration/resources/regression/java8/boogie/byteback.dummy.condition.Boolean.bpl
@@ -1,61 +1,5 @@
-// -------------------------------------------------------------------
-// Heap model
-// -------------------------------------------------------------------
-type Reference;
-
-const ~null: Reference;
-
-type Field a;
-type Store = [Reference]<a>[Field a]a;
-
-var ~heap: Store;
-
-function ~read<a>(h: Store, r: Reference, f: Field a) returns (a)
-{ h[r][f] }
-
-function ~update<a>(h: Store, r: Reference, f: Field a, v: a) returns (Store)
-{ h[r := h[r][f := v]] }
-
-// -------------------------------------------------------------------
-// Binary operators
-// -------------------------------------------------------------------
-function ~cmp<a>(a, a) returns (int);
-
-axiom (forall i: int, j: int :: i < j ==> ~cmp(i, j) == -1);
-axiom (forall i: int, j: int :: i > j ==> ~cmp(i, j) == 1);
-axiom (forall i: int, j: int :: i == j ==> ~cmp(i, j) == 0);
-
-axiom (forall i: real, j: real :: i < j ==> ~cmp(i, j) == -1);
-axiom (forall i: real, j: real :: i > j ==> ~cmp(i, j) == 1);
-axiom (forall i: real, j: real :: i == j ==> ~cmp(i, j) == 0);
-
-// -------------------------------------------------------------------
-// Casting operators
-// -------------------------------------------------------------------
-
-// Casting between primitive types
-function ~int<a>(a) returns (int);
-
-// bool -> int
-axiom ~int(false) == 0;
-axiom ~int(true) == 1;
-
-function eq(~heap: Store, a: int, b: int) returns (bool) { a == b }
-
-function implies(~heap: Store, a: bool, b: bool) returns (bool) { a ==> b }
-
-function not(~heap: Store, a: bool) returns (bool) { !a }
-
-// real -> int
-// TODO
-
-function ~real<a>(a) returns (real);
-
-// int -> real
-// TODO
-
 procedure byteback.dummy.condition.Boolean.shortCircuitingAnd#boolean#boolean#(a: bool, b: bool) returns (~ret: bool)
-  ensures implies(~heap, a && b, ~ret);
+  ensures ~implies(~heap, a && b, ~ret);
 {
   var $stack2: bool;
 
@@ -80,7 +24,7 @@ label3:
 }
 
 procedure byteback.dummy.condition.Boolean.shortCircuitingOr#boolean#boolean#(a: bool, b: bool) returns (~ret: bool)
-  ensures implies(~heap, a || b, ~ret);
+  ensures ~implies(~heap, a || b, ~ret);
 {
   var $stack2: bool;
 
@@ -106,7 +50,7 @@ label3:
 }
 
 procedure byteback.dummy.condition.Boolean.shortCircuitingNot#boolean#(a: bool) returns (~ret: bool)
-  ensures implies(~heap, a, not(~heap, ~ret));
+  ensures ~implies(~heap, a, ~not(~heap, ~ret));
 {
   var $stack1: bool;
 
