byteback-core/src/integration/resources/regression/java8/boogie/byteback.dummy.condition.Counter.bpl
@@ -1,57 +1,3 @@
-// -------------------------------------------------------------------
-// Heap model
-// -------------------------------------------------------------------
-type Reference;
-
-const ~null: Reference;
-
-type Field a;
-type Store = [Reference]<a>[Field a]a;
-
-var ~heap: Store;
-
-function ~read<a>(h: Store, r: Reference, f: Field a) returns (a)
-{ h[r][f] }
-
-function ~update<a>(h: Store, r: Reference, f: Field a, v: a) returns (Store)
-{ h[r := h[r][f := v]] }
-
-// -------------------------------------------------------------------
-// Binary operators
-// -------------------------------------------------------------------
-function ~cmp<a>(a, a) returns (int);
-
-axiom (forall i: int, j: int :: i < j ==> ~cmp(i, j) == -1);
-axiom (forall i: int, j: int :: i > j ==> ~cmp(i, j) == 1);
-axiom (forall i: int, j: int :: i == j ==> ~cmp(i, j) == 0);
-
-axiom (forall i: real, j: real :: i < j ==> ~cmp(i, j) == -1);
-axiom (forall i: real, j: real :: i > j ==> ~cmp(i, j) == 1);
-axiom (forall i: real, j: real :: i == j ==> ~cmp(i, j) == 0);
-
-// -------------------------------------------------------------------
-// Casting operators
-// -------------------------------------------------------------------
-
-// Casting between primitive types
-function ~int<a>(a) returns (int);
-
-// bool -> int
-axiom ~int(false) == 0;
-axiom ~int(true) == 1;
-
-procedure ~new() returns (~ret: Reference);
-
-function eq(~heap: Store, a: int, b: int) returns (bool) { a == b }
-
-function implies(~heap: Store, a: bool, b: bool) returns (bool) { a ==> b }
-
-function not(~heap: Store, a: bool) returns (bool) { !a }
-
-// real -> int
-// TODO
-function ~real<a>(a) returns (real);
-
 const byteback.dummy.condition.Counter.count: Field int;
 
 procedure byteback.dummy.condition.Counter.main##() returns ()
@@ -59,34 +5,34 @@ procedure byteback.dummy.condition.Counter.main##() returns ()
   var $stack1: Reference;
   call $stack1 := ~new();
   call byteback.dummy.condition.Counter.$init$##($stack1);
-  assert eq(~heap, ~read(~heap, $stack1, byteback.dummy.condition.Counter.count), 0);
+  assert ~eq(~heap, ~read(~heap, $stack1, byteback.dummy.condition.Counter.count), 0);
   call byteback.dummy.condition.Counter.increment##($stack1);
-  assert eq(~heap, ~read(~heap, $stack1, byteback.dummy.condition.Counter.count), 1);
+  assert ~eq(~heap, ~read(~heap, $stack1, byteback.dummy.condition.Counter.count), 1);
   call byteback.dummy.condition.Counter.countTo10##($stack1);
-  assert eq(~heap, ~read(~heap, $stack1, byteback.dummy.condition.Counter.count), 11);
+  assert ~eq(~heap, ~read(~heap, $stack1, byteback.dummy.condition.Counter.count), 11);
   call byteback.dummy.condition.Counter.countTo10Indirectly##($stack1);
-  assert eq(~heap, ~read(~heap, $stack1, byteback.dummy.condition.Counter.count), 21);
+  assert ~eq(~heap, ~read(~heap, $stack1, byteback.dummy.condition.Counter.count), 21);
   return;
 }
 
 procedure byteback.dummy.condition.Counter.$init$##(this: Reference) returns ()
-  ensures eq(~heap, ~read(~heap, this, byteback.dummy.condition.Counter.count), 0);
+  ensures ~eq(~heap, ~read(~heap, this, byteback.dummy.condition.Counter.count), 0);
 {
   call java.lang.Object.$init$##(this);
   ~heap := ~update(~heap, this, byteback.dummy.condition.Counter.count, 0);
   return;
 } 
 
-procedure byteback.dummy.condition.Counter.increment##(this : Reference) returns ()
-  ensures eq(~heap, ~read(~heap, this, byteback.dummy.condition.Counter.count), old(~read(~heap, this, byteback.dummy.condition.Counter.count)) + 1);
+procedure byteback.dummy.condition.Counter.increment##(this: Reference) returns ()
+  ensures ~eq(~heap, ~read(~heap, this, byteback.dummy.condition.Counter.count), old(~read(~heap, this, byteback.dummy.condition.Counter.count)) + 1);
 {
   ~heap := ~update(~heap, this, byteback.dummy.condition.Counter.count,
     ~read(~heap, this, byteback.dummy.condition.Counter.count) + 1);
   return;
 }
 
-procedure byteback.dummy.condition.Counter.countTo10##(this : Reference) returns ()
-  ensures eq(~heap, ~read(~heap, this, byteback.dummy.condition.Counter.count),
+procedure byteback.dummy.condition.Counter.countTo10##(this: Reference) returns ()
+  ensures ~eq(~heap, ~read(~heap, this, byteback.dummy.condition.Counter.count),
     old(~read(~heap, this, byteback.dummy.condition.Counter.count)) + 10);
 {
   var i: int;
@@ -106,8 +52,8 @@ label1:
   return;
 }
 
-procedure byteback.dummy.condition.Counter.countTo10Indirectly##(this : Reference) returns ()
-  ensures eq(~heap, ~read(~heap, this, byteback.dummy.condition.Counter.count),
+procedure byteback.dummy.condition.Counter.countTo10Indirectly##(this: Reference) returns ()
+  ensures ~eq(~heap, ~read(~heap, this, byteback.dummy.condition.Counter.count),
     old(~read(~heap, this, byteback.dummy.condition.Counter.count)) + 10);
 {
   var i: int;
