byteback-core/src/integration/resources/regression/java8/boogie/byteback.dummy.function.Simple.bpl
@@ -1,9 +1,9 @@
 function byteback.dummy.function.Simple.universalQuantifier##(~heap: Store) returns (bool)
 {
-  (forall i : int :: true)
+  (forall i: int :: true)
 }
 
 function byteback.dummy.function.Simple.existentialQuantifier##(~heap: Store) returns (bool)
 {
-  (exists i : int :: true)
+  (exists i: int :: true)
 }
